Work in progress; adding encoding of lambdas

src/smtencoding/FStarC.SMTEncoding.Encode.fst
@@ -379,7 +379,7 @@ let primitive_type_axioms : env -> lident -> string -> term -> list decl =
         in
         [Util.mkAssume(mkForall (Env.get_range env) ([[inversion_t]], [uu;tt], mkImp(valid, body)), Some "inversion interpretation", "inversion-interp")]
    in
-   let mk_with_type_axiom : env -> string -> term -> list decl = fun env with_type tt ->
+   let mk_with_type_axiom : env -> string -> term -> list decl = fun env with_type _tt ->
         (* (assert (forall ((u Universe) (t Term) (e Term))
                            (! (and (= (Prims.with_type u t e)
                                        e)
@@ -402,6 +402,69 @@ let primitive_type_axioms : env -> lident -> string -> term -> list decl =
                        Some "with_type primitive axiom",
                        "@with_type_primitive_axiom")] //the "@" in the name forces it to be retained even when the contex is pruned
    in
+   let mk_has_eq_refine : env -> string -> term -> list decl = fun env has_eq _has_eq_tt ->
+      (* (assert (forall ((u Universe) (base Term) (refine (=> Term Bool)))
+                         (! (iff (Prims.hasEq u base) (Prims.hasEq u (Tm_refine base refine))))
+                            :pattern ((Prims.hasEq u (Tm_refine base refine)))
+                            :qid tm_refine_has_eq))) *)
+        let uu = mk_fv ("u", univ_sort) in
+        let u = mkFreeV uu in
+        let bb = mk_fv ("base", Term_sort) in
+        let base = mkFreeV bb in
+        let rr = mk_fv ("refine", Arrow (Term_sort, Bool_sort)) in
+        let refine = mkFreeV rr in
+        let has_eq_base = mkApp(has_eq, [u; base]) in
+        let has_eq_refine = mkApp(has_eq, [u; mkTm_refinement Range.dummyRange base refine]) in
+        [Util.mkAssume(mkForall' (Env.get_range env) 
+                                 ([[has_eq_refine]], None, [uu; bb; rr],
+                                   mkIff (has_eq_base, has_eq_refine)),
+                       Some "has_eq_refine axiom",
+                       "has_eq_refine")]
+   in
+   let mk_forall_interp  : env -> string -> term -> list decl  = fun env forall_lid _ ->
+    let uu = mk_fv ("u", univ_sort) in
+    let u = mkFreeV uu in
+    let tt = mk_fv ("t", Term_sort) in
+    let t = mkFreeV tt in
+    let bb = mk_fv ("body", Term_sort) in
+    let body = mkFreeV bb in
+    let lhs = mk_Valid (mkApp(forall_lid, [u;t;body])) in
+    let xx = mk_fv ("x", Term_sort) in
+    let x = mkFreeV xx in
+    let rhs = 
+        mkForall' (Env.get_range env) ([], None, [xx], 
+          mkImp (
+            mk_HasType x t, 
+            mk_Valid (mk_ApplyTT body x))
+        )
+    in
+    [Util.mkAssume(mkForall' (Env.get_range env)
+                             ([[lhs]], None, [uu; tt; bb], mkIff (lhs, rhs)),
+                      Some "l_forall_interp",
+                      "l_forall_interp")]
+   in
+   let mk_exists_interp  : env -> string -> term -> list decl  = fun env exists_lid _ ->
+    let uu = mk_fv ("u", univ_sort) in
+    let u = mkFreeV uu in
+    let tt = mk_fv ("t", Term_sort) in
+    let t = mkFreeV tt in
+    let bb = mk_fv ("body", Term_sort) in
+    let body = mkFreeV bb in
+    let lhs = mk_Valid (mkApp(exists_lid, [u;t;body])) in
+    let xx = mk_fv ("x", Term_sort) in
+    let x = mkFreeV xx in
+    let rhs = 
+      mkExists (Env.get_range env) ([], [xx], 
+        mkAnd(
+          mk_HasType x t,
+          mk_Valid (mk_ApplyTT body x))
+        )
+    in
+    [Util.mkAssume(mkForall' (Env.get_range env)
+                             ([[lhs]], None, [uu; tt; bb], mkIff (lhs, rhs)),
+                      Some "l_exists_interp",
+                      "l_exists_interp")]
+   in
    let prims =  [(Const.unit_lid,   mk_unit);
                  (Const.bool_lid,   mk_bool);
                  (Const.int_lid,    mk_int);
@@ -415,10 +478,11 @@ let primitive_type_axioms : env -> lident -> string -> term -> list decl =
                  (Const.imp_lid,    mk_imp_interp);
                  (Const.iff_lid,    mk_iff_interp);
                  (Const.not_lid,    mk_not_interp);
-                 //(Const.forall_lid, mk_forall_interp);
-                 //(Const.exists_lid, mk_exists_interp);
+                //  (Const.forall_lid, mk_forall_interp);
+                //  (Const.exists_lid, mk_exists_interp);
                  (Const.range_lid,  mk_range_interp);
                  (Const.inversion_lid,mk_inversion_axiom);
+                 (Const.haseq_lid, mk_has_eq_refine)
                 ] in
     (fun (env:env) (t:lident) (s:string) (tt:term) ->
         match Option.find (fun (l, _) -> lid_equals l t) prims with
